thys/core.thy
@@ -3,34 +3,98 @@ imports
   core_export
 begin
 
+definition "all_option P = case_option False P"
+
+lemma all_option_Some[simp]: "all_option P (Some x) = P x"
+by (simp add: all_option_def)
+
+lemma all_option_None[simp]: "\<not>all_option P None"
+by (simp add: all_option_def)
+
+lemma all_optionE[elim!]:
+  assumes "all_option P x"
+  obtains x' where "x = Some x'" "P x'"
+using assms by (cases x; simp)
+
+lemma all_option_comp: "all_option (P \<circ> f) x = all_option P (map_option f x)"
+by (cases x; simp)
+
+lemma all_option_eq: "all_option (\<lambda>x. x = y) x \<longleftrightarrow> x = Some y"
+by (cases x; simp)
+
+theorem while_opt_rule_lemma:
+  assumes invariant: "!!s. P s ==> b s ==> P (c s)"
+    and terminate: "!!s. P s ==> \<not> b s ==> Q s"
+    and wf: "wf {(t, s). P s \<and> b s \<and> t = c s}"
+  shows "P s \<Longrightarrow> all_option Q (while_option b c s)"
+  using wf
+  apply (induct s)
+  apply simp
+  apply (subst while_option_unfold)
+  apply (simp add: invariant terminate all_option_def)
+  done
+
+theorem while_opt_rule:
+  "[| P s;
+      !!s. [| P s; b s  |] ==> P (c s);
+      !!s. [| P s; \<not> b s  |] ==> Q s;
+      wf r;
+      !!s. [| P s; b s  |] ==> (c s, s) \<in> r |] ==>
+   all_option Q (while_option b c s)"
+  apply (rule while_opt_rule_lemma)
+     prefer 4 apply assumption
+    apply blast
+   apply blast
+  apply (erule wf_subset)
+  apply blast
+  done
+
 lemma loop_rule:
   assumes "P s"
   assumes "\<And>s s'. P s \<Longrightarrow> l s = (s',True) \<Longrightarrow> P s'" "\<And>s s'. P s \<Longrightarrow> l s = (s',False) \<Longrightarrow> Q s'"
   assumes "wf r" "\<And>s s'. P s \<Longrightarrow> l s = (s',True) \<Longrightarrow> (s', s) \<in> r"
-  shows "Q (loop l s)"
+  shows "all_option Q (loop l s)"
 proof-
   let ?r' = "{((s\<^sub>1, l s\<^sub>1), (s\<^sub>2, l s\<^sub>2)) | s\<^sub>1 s\<^sub>2. (s\<^sub>1,s\<^sub>2) \<in> r}"
   have "wf ?r'"
     by (rule compat_wf[where f=fst, OF _ assms(4)]) (auto simp: compat_def)
+
   show ?thesis
-    unfolding loop_def
-    by (rule while_rule[where P="\<lambda>(s,s'). P s \<and> s' = l s" and r="?r'", OF _ _ _ `wf ?r'`]) (auto simp: assms)
+  unfolding loop_def all_option_comp[symmetric]
+  by (rule while_opt_rule[where P="\<lambda>(s,s'). P s \<and> l s = s'", OF _ _ _ `wf ?r'`])
+     (auto simp: assms pred_option_def)
 qed
 
-declare split_def[simp] Let_def[simp]
+lemma loop'_rule:
+  assumes "P s"
+  assumes "\<And>s. P s \<Longrightarrow> l s \<noteq> None" "\<And>s s'. P s \<Longrightarrow> l s = Some (s',True) \<Longrightarrow> P s'" "\<And>s s'. P s \<Longrightarrow> l s = Some (s',False) \<Longrightarrow> Q s'"
+  assumes "wf r" "\<And>s s'. P s \<Longrightarrow> l s = Some (s',True) \<Longrightarrow> (s', s) \<in> r"
+  shows "all_option Q (loop' l s)"
+proof-
+  let ?r' = "{(Some s\<^sub>1, Some s\<^sub>2) | s\<^sub>1 s\<^sub>2. (s\<^sub>1,s\<^sub>2) \<in> r}"
+  have "wf ?r'"
+    by (rule compat_wf[where f=the, OF _ assms(5)]) (auto simp: compat_def)
+
+  show ?thesis
+  by (cut_tac loop_rule[where P="all_option P" and Q="all_option Q" and s="Some s", OF _ _ _ `wf ?r'`])
+     (auto simp: loop'_def all_option_def pred_option_def Option.bind_def assms(1,2,6) intro: assms(3,4) split: option.splits)
+qed
+
+declare Let_def[simp]
 
 lemma loop_range_u32:
   assumes "P l res\<^sub>0"
   assumes "\<And>i res. \<lbrakk>l \<le> i; i < r; P i res\<rbrakk> \<Longrightarrow> P (Suc i) (f i res)"
-  shows "P (max l r) (fst (loop (\<lambda>(res, iter).
-                  let (t6, iter) = core_iter_ops_Range_A__Iterator_next core_num_u32_One core_iter_u32_Step core_ops___b_u32_Add___a_u32 iter
-                  in case t6 of core_option_Option_None \<Rightarrow> ((res, iter), False)
-                     | core_option_Option_Some i \<Rightarrow> ((f i res, iter), True))
-         (res\<^sub>0, core_ops_Range.make l r)))"
-apply (rule loop_rule[where P="\<lambda>s. case s of (res, iter) \<Rightarrow>
+  shows "all_option (P (max l r) \<circ> fst) (loop' (\<lambda>(res, iter).
+                  do (t6, iter) \<leftarrow> (core_iter_ops_Range_A__Iterator_next (core_num_u32_One) (core_iter_u32_Step) (core_ops___b_u32_Add___a_u32) iter);
+                  case t6 of core_option_Option_None \<Rightarrow> Some ((res, iter), False)
+                     | core_option_Option_Some i \<Rightarrow> Some ((f i res, iter), True))
+         (res\<^sub>0, core_ops_Range.make l r))"
+apply (rule loop'_rule[where P="\<lambda>s. case s of (res, iter) \<Rightarrow>
     let i = core_ops_Range_start iter in
     l \<le> i \<and> i \<le> max l r \<and> core_ops_Range_end iter = r \<and> P i res"])
-    apply (auto simp: core_ops_Range.make_def assms(1))[1]
+     apply (auto simp: core_ops_Range.make_def assms(1))[1]
+    apply auto[1]
    apply (auto split: option.splits split_if_asm intro!: assms(2))[1]
   apply (auto simp: max_absorb1 max_absorb2 le_max_iff_disj not_less split: option.splits split_if_asm)[1]
  apply (rule wf_measure[of "\<lambda>s. case s of (_,iter) \<Rightarrow> core_ops_Range_end iter - core_ops_Range_start iter"])
@@ -39,15 +103,13 @@ done
 
 lemma loop_range_u32':
   assumes "body = (\<lambda>(res, iter).
-                  let (t6, iter) = core_iter_ops_Range_A__Iterator_next core_num_u32_One core_iter_u32_Step core_ops___b_u32_Add___a_u32 iter
-                  in case t6 of core_option_Option_None \<Rightarrow> ((res, iter), False)
-                     | core_option_Option_Some i \<Rightarrow> ((f i res, iter), True))"
-  assumes "P (max l r) (fst (loop body (res\<^sub>0, core_ops_Range.make l r))) \<Longrightarrow> P'"
+                  do (t6, iter) \<leftarrow> core_iter_ops_Range_A__Iterator_next core_num_u32_One core_iter_u32_Step core_ops___b_u32_Add___a_u32 iter;
+                  case t6 of core_option_Option_None \<Rightarrow> Some ((res, iter), False)
+                     | core_option_Option_Some i \<Rightarrow> Some ((f i res, iter), True))"
+  assumes "\<And>x. P (max l r) (fst x) \<Longrightarrow> P' (Some x)"
   assumes "P l res\<^sub>0"
   assumes "\<And>i res. \<lbrakk>l \<le> i; i < r; P i res\<rbrakk> \<Longrightarrow> P (Suc i) (f i res)"
-  shows "P'"
-apply (rule assms(2))
-unfolding assms(1)
-by (rule loop_range_u32; rule assms(3-4); assumption)
+  shows "P' (loop' body (res\<^sub>0, core_ops_Range.make l r))"
+by (cut_tac loop_range_u32[of P l res\<^sub>0 r f]) (auto simp: assms)
 
 end
