thys/core_pre.thy
@@ -2,17 +2,35 @@ theory core_pre
 imports Main "~~/src/HOL/Library/While_Combinator"
 begin
 
-definition loop :: "('state \<Rightarrow> 'state \<times> bool) \<Rightarrow> 'state \<Rightarrow> 'state" where
-  "loop l s = (let (s,s',c) = while (\<lambda>(s,s',c). c) (\<lambda>(s,s',c). (s',(l s'))) (s,(l s)) in s')"
+nonterminal dobinds and dobind
+syntax
+  "_bind"       :: "[pttrn, 'a] => dobind"              ("(2_ \<leftarrow>/ _)" 10)
+  "_Do"         :: "[dobind, 'a] => 'a"                 ("(do (_)/; (_))" [0, 10] 10)
 
+translations
+  "do x \<leftarrow> a; e"        == "CONST Option.bind a (%x. e)"
+
+definition loop :: "('state \<Rightarrow> 'state \<times> bool) \<Rightarrow> 'state \<Rightarrow> 'state option" where
+  "loop l s \<equiv> map_option (\<lambda>(s,s',c). s')
+    (while_option (\<lambda>(s,s',c). c) (\<lambda>(s,s',c). (s',(l s'))) (s,(l s)))"
+
+definition loop' :: "('state \<Rightarrow> ('state \<times> bool) option) \<Rightarrow> 'state \<Rightarrow> 'state option" where
+  "loop' l s = Option.bind (
+    loop (\<lambda>s. case s of
+      None \<Rightarrow> (None, False)
+    | Some s \<Rightarrow> (case l s of
+        None \<Rightarrow> (Some s, False)
+      | Some (s',c) \<Rightarrow> (Some s',c)))
+    (Some s)
+  ) id"
 
 type_synonym u32 = nat
 type_synonym usize = nat
 
 definition[simp]: "u32_to_usize = id"
 
-definition[simp]: "core_num_u32_overflowing_add x y = (x + y, False)"
+definition[simp]: "core_num_u32_overflowing_add x y = Some (x + y, False)"
 
-definition[simp]: "core_mem_swap x y = ((),y,x)"
+definition[simp]: "core_mem_swap x y = Some ((),y,x)"
 
 end
