ROOT
@@ -2,7 +2,8 @@ session "rustabelle" = "HOL" +
   options [document = pdf, document_output = "output"]
   theories [document = false]
     "~~/src/HOL/Library/While_Combinator"
+    "thys/core_export"
   theories
-    "prove/examples"
+    "thys/examples"
   document_files
     "root.tex"
